demo/fib/Fib23proof_old.v
@@ -1,0 +1,275 @@
+Require Import CoqlibC Maps Postorder.
+Require Import AST Linking.
+Require Import ValuesC MemoryC GlobalenvsC Events Smallstep.
+Require Import Op ClightC.
+Require Import CtypesC CtypingC.
+Require Import sflib.
+Require Import IntegersC.
+
+Require Import Simulation.
+Require Import Skeleton Mod ModSem SimMod SimModSemLift SimSymb SimMemLift MatchSimModSemExcl.
+Require SoundTop.
+Require SimMemId.
+Require Import Any.
+Require Import SIR.
+Require Import FibHeader.
+Require Import Fib3_old.
+Require Import Fib2.
+Require Import ModSemProps.
+Require Import Program.
+Require Import SIRProps.
+
+Set Implicit Arguments.
+
+
+
+
+
+
+
+
+
+
+Lemma bind_unwrapU
+      E `{EventE -< E} R S
+      (r: option R) r'
+      (k: R -> itree E S)
+      (SOME: r = Some r')
+  :
+    ` x : _ <- unwrapU r;; k x = k r'.
+Proof.
+  rewrite SOME. cbn. eapply bind_ret_l.
+Qed.
+
+Lemma bind_unwrapN
+      E `{EventE -< E} R S
+      (r: option R) r'
+      (k: R -> itree E S)
+      (SOME: r = Some r')
+  :
+    ` x : _ <- unwrapN r;; k x = k r'.
+Proof.
+  rewrite SOME. cbn. eapply bind_ret_l.
+Qed.
+
+Lemma bind_assume
+      E `{EventE -< E} R
+      (P: Prop)
+      (prf: P)
+      (k: itree E R)
+  :
+    assume P ;; k = k.
+Proof.
+  unfold assume. des_ifs. rewrite bind_ret_l. ss.
+Qed.
+
+Lemma bind_guarantee
+      E `{EventE -< E} R
+      (P: Prop)
+      (prf: P)
+      (k: itree E R)
+  :
+    guarantee P ;; k = k.
+Proof.
+  unfold guarantee. des_ifs. rewrite bind_ret_l. ss.
+Qed.
+
+
+
+
+
+
+
+Ltac step := gstep; econs; et.
+Ltac step_assume := match goal with
+                    | |- context[assume ?P ;; _] =>
+                      (*** I want to unfold only the "first" assume.
+Maybe we should use notation instead, so that we can avoid this weird "unfold"? ***)
+                      first[
+                          unfold assume at 5|
+                          unfold assume at 4|
+                          unfold assume at 3|
+                          unfold assume at 2|
+                          unfold assume at 1|
+                          unfold assume at 0
+                        ];
+                      let name := fresh "T" in
+                      destruct (ClassicalDescription.excluded_middle_informative P) as [name|name]; cycle 1; [
+                        unfold triggerUB; rewrite bind_vis (*** <---------- this is counter-intuitive. Any good idea? ***);
+                        try step|]
+                    end
+.
+Ltac step_unwrapN := match goal with
+                     | |- context[unwrapN ?ox ;; _] =>
+                       (*** I want to unfold only the "first" assume.
+Maybe we should use notation instead, so that we can avoid this weird "unfold"? ***)
+                       first[
+                           unfold unwrapN at 5|
+                           unfold unwrapN at 4|
+                           unfold unwrapN at 3|
+                           unfold unwrapN at 2|
+                           unfold unwrapN at 1|
+                           unfold unwrapN at 0
+                         ];
+                       let name := fresh "T" in
+                       destruct ox eqn:name; cycle 1
+                     end
+.
+Ltac step_guaranteeK := match goal with
+                        | |- context[guaranteeK ?P ;; _] =>
+                          (*** I want to unfold only the "first" assume.
+Maybe we should use notation instead, so that we can avoid this weird "unfold"? ***)
+                          first[
+                              unfold guaranteeK at 5|
+                              unfold guaranteeK at 4|
+                              unfold guaranteeK at 3|
+                              unfold guaranteeK at 2|
+                              unfold guaranteeK at 1|
+                              unfold guaranteeK at 0
+                            ];
+                          destruct (ClassicalDescription.excluded_middle_informative P); cycle 1
+                        | |- context[guaranteeK ?P ?Q] =>
+                          (*** I want to unfold only the "first" assume.
+Maybe we should use notation instead, so that we can avoid this weird "unfold"? ***)
+                          first[
+                              unfold guaranteeK at 5|
+                              unfold guaranteeK at 4|
+                              unfold guaranteeK at 3|
+                              unfold guaranteeK at 2|
+                              unfold guaranteeK at 1|
+                              unfold guaranteeK at 0
+                            ];
+                          destruct (ClassicalDescription.excluded_middle_informative (P Q)); cycle 1
+                        end
+.
+Ltac step_guarantee := match goal with
+                    | |- context[guarantee ?P ;; _] =>
+                      (*** I want to unfold only the "first" guarantee.
+Maybe we should use notation instead, so that we can avoid this weird "unfold"? ***)
+                      first[
+                          unfold guarantee at 5|
+                          unfold guarantee at 4|
+                          unfold guarantee at 3|
+                          unfold guarantee at 2|
+                          unfold guarantee at 1|
+                          unfold guarantee at 0
+                        ];
+                      let name := fresh "T" in
+                      destruct (ClassicalDescription.excluded_middle_informative P) as [name|name]; cycle 1; [
+                        unfold triggerNB; rewrite bind_vis (*** <---------- this is counter-intuitive. Any good idea? ***);
+                        try step|]
+                    end
+.
+
+
+
+(* Hint Unfold assume guarantee assumeK guaranteeK triggerUB triggerNB unwrapU unwrapN. *)
+Theorem correct: rusc defaultR [Fib3_old.module: Mod.t] [Fib2.module: Mod.t].
+Proof.
+  assert(AA := range_to_nat).
+  assert(SUCPRED := succ_pred).
+
+  eapply SIRLocal.correct with (SO := eq); ss.
+  prog_tac.
+  ginit. { i. eapply cpn2_wcompat; eauto with paco. }
+  unfold Fib3_old.f_fib, f_fib.
+  step_assume.
+  unfold precond, parse_arg in *. des. des_ifs_safe. irw. rewrite T. irw.
+  destruct n eqn:U.
+  { rewrite bind_ret_l. clarify.
+    assert(i = Int.zero).
+    { unfold to_nat_opt in *. des_ifs.
+      assert((Int.signed i) = 0).
+      { apply Z2Nat.inj; ss. }
+      apply func_app with (f:=Int.repr) in H. rewrite Int.repr_signed in H. ss.
+    }
+    clarify. rewrite Int.eq_true. step_guaranteeK.
+    { unfold postcond, NW in *. des_ifs; repeat (Psimpl; des; ss; et). clarify. }
+    step.
+  }
+  destruct n0 eqn:V.
+  { rewrite bind_ret_l. u.
+    assert(i = Int.one).
+    { unfold to_nat_opt in *. des_ifs.
+      assert((Int.signed i) = 1).
+      { apply Z2Nat.inj; ss. }
+      apply func_app with (f:=Int.repr) in H. rewrite Int.repr_signed in H. ss.
+    }
+    clarify. rewrite Int.eq_true. step_guaranteeK.
+    { des_ifs; repeat (Psimpl; des; ss; et). }
+    step.
+  }
+  Fail rewrite bind_unwrapN. (*** <---------- TODO: FIXIT ***)
+  assert(R: Int.min_signed <= Z.of_nat n0 <= Int.max_signed).
+  { unfold to_nat_opt in *. des_ifs.
+    generalize (Nat2Z.is_nonneg (S n1)); i. generalize Int.min_signed_neg; i.
+    generalize (Int.signed_range i); i.
+    split; try xomega.
+    assert(Z.of_nat (S (S n1)) <= Int.max_signed).
+    { rewrite <- H0. rewrite Z2Nat.id; ss. xomega. }
+    xomega.
+  }
+  assert(R0: Int.min_signed <= Z.of_nat n <= Int.max_signed).
+  { unfold to_nat_opt in *. des_ifs.
+    generalize (Nat2Z.is_nonneg (S n1)); i. generalize Int.min_signed_neg; i.
+    generalize (Int.signed_range i); i.
+    split; try xomega.
+    assert(Z.of_nat (S (S n1)) <= Int.max_signed).
+    { rewrite <- H0. rewrite Z2Nat.id; ss. xomega. }
+    xomega.
+  }
+  (* destruct (to_nat_opt (of_nat n0)) eqn:W; cbn; cycle 1. *)
+  (* { exfalso. unfold to_nat_opt in *. des_ifs. psimpl. unfold of_nat in *. rewrite Int.signed_repr in *; ss. xomega. } *)
+  assert(~Int.eq i Int.zero).
+  { ii. apply_all_once Int.same_if_eq. clarify. }
+  assert(~Int.eq i Int.one).
+  { ii. apply_all_once Int.same_if_eq. clarify. }
+  des_ifs_safe.
+  rewrite ! AA; try lia. cbn.
+  step_guarantee.
+  { clear - R T0. u in T0. des_ifs. lia. }
+  irw.
+  step_guarantee.
+  { Psimpl. contradict T1; eauto. }
+  irw.
+  clear_tac. clear T0.
+  assert(U: of_nat n1 = Int.sub i (Int.repr 2)).
+  { unfold to_nat_opt in *. des_ifs. unfold of_nat.
+    eapply SUCPRED in H0; des.
+    eapply SUCPRED in H0; des. ss. clarify.
+    (* rewrite <- Nat.sub_add_distr. ss. *)
+    rewrite Nat2Z.inj_sub; ss. rewrite Nat2Z.inj_sub; ss. rewrite <- Z.sub_add_distr; ss.
+    rewrite <- Int_sub_repr. f_equal. rewrite Z2Nat.id; ss. rewrite Int.repr_signed; ss.
+  }
+  rewrite <- U. step.
+  sii S. r in S. des_ifs_safe. des. clarify.
+  rewrite bind_bind.
+  (* unfold assume at 2. *)
+  step_assume. des. clarify.
+  rewrite bind_ret_l.
+  rewrite bind_bind.
+  assert(V: of_nat (S n) = Int.sub i (Int.repr 1)).
+  { unfold to_nat_opt in *. des_ifs. unfold of_nat.
+    eapply SUCPRED in H0; des.
+    eapply SUCPRED in H0; des. ss. clarify.
+    rewrite Nat.sub_1_r. rewrite Nat.succ_pred; ss; cycle 1.
+    { intro X. rewrite X in *. inv H2. }
+    rewrite Nat2Z.inj_sub; ss.
+    rewrite <- Int_sub_repr. f_equal. rewrite Z2Nat.id; ss. rewrite Int.repr_signed; ss.
+  }
+  cbn.
+  step_guarantee.
+  { clear - R1 T0. u in T0. des_ifs. lia. }
+  irw.
+  step_guarantee.
+  { eapply Classical_Pred_Type.not_ex_all_not in T1. contradict T1; eauto. }
+  irw. rewrite V. step.
+  sii S. r in S. des_ifs_safe; des; clarify.
+  irw.
+  step_assume.
+  des; des_ifs_safe. irw.
+  step_guaranteeK.
+  { unfold postcond, parse_arg in *. unfold NW in *. des_ifs. repeat (Psimpl; des; ss; et). }
+  rewrite fib_nat_recurse.
+  unfold of_nat. rewrite Int_add_repr. rewrite Nat2Z.inj_add. clear_tac. step.
+Qed.
