demo/fib/Fib3_old.v
@@ -19,26 +19,27 @@ Definition f_fib (oh0: owned_heap) (m0: mem) (vs0: list val):
   itree (E owned_heap) (owned_heap * (mem * val)) :=
   assume (precond oh0 m0 vs0) ;;
 
-  match vs0 with
-  | [Vint n] =>
-    if Int.eq n Int.zero
-    then Ret (oh0, (m0, (Vint Int.zero)))
-    else
-      if Int.eq n Int.one
-      then Ret (oh0, (m0, (Vint Int.one)))
-      else
-        let vs0 := [Vint (Int.sub n (Int.repr 2))] in
-        guarantee (precond oh0 m0 vs0) ;;
-        '(oh1, (m1, y1)) <- trigger (ICall _fib oh0 m0 vs0) ;;
-        (assume (postcond oh0 m0 vs0 (oh1, (m1, y1)))) ;;
+  `n: nat <- (unwrapN (parse_arg oh0 m0 vs0)) ;;
+    match n with
+    | O => Ret (oh0, (m0, (Vint Int.zero)))
+    | S O => Ret (oh0, (m0, (Vint Int.one)))
+    | S (S m) =>
+      let vs0 := [Vint (of_nat m)] in
 
-        let vs1 := [Vint (Int.sub n (Int.repr 1))] in
-        guarantee (precond oh1 m1 vs1) ;;
-        '(oh2, (m2, y2)) <- trigger (ICall _fib oh1 m1 vs1) ;;
-        (assume (postcond oh1 m1 vs1 (oh2, (m2, y2)))) ;;
-        Ret (oh2, (m2, Val.add y1 y2))
-  | _ => triggerUB
-  end
+      guarantee (of_nat_opt m) ;;
+      guarantee (precond oh0 m0 vs0) ;;
+      '(oh1, (m1, y1)) <- trigger (ICall _fib oh0 m0 vs0) ;;
+      (assume (postcond oh0 m0 vs0 (oh1, (m1, y1)))) ;;
+
+      let vs1 := [Vint (of_nat (S m))] in
+
+      guarantee (of_nat_opt (S m)) ;;
+      guarantee (precond oh1 m1 vs1) ;;
+      '(oh2, (m2, y2)) <- trigger (ICall _fib oh1 m1 vs1) ;;
+      (assume (postcond oh1 m1 vs1 (oh2, (m2, y2)))) ;;
+
+      Ret (oh2, (m2, Vint (of_nat (fib_nat n))))
+    end
 
   >>= guaranteeK (postcond oh0 m0 vs0)
 .
